lunarlander/nonlinear.thy
@@ -12,6 +12,8 @@ definition y :: exp where
 definition z :: exp where
   "z == RVar ''parz''"
 
+definition a :: exp where
+  "a == RVar ''para''"
 
 consts Inv :: fform
 
@@ -85,6 +87,106 @@ apply (cut_tac allcons3)
 
 
 
+definition cons41 :: fform where "cons41 \<equiv> (x [=] Real 1 [&] y [=] Real 0 [&] z [=] Real 0) [\<longrightarrow>] Inv"
+definition cons42 :: fform where "cons42 \<equiv> Inv [&] close(x[**]2[+]y[**]2[+]z[**]2[=] Real 1)[\<longrightarrow>] (x [\<le>] Real 1 [&] z[\<le>] Real 0)"
+definition cons43 :: fform where "cons43 \<equiv> exeFlow(<[''parx'',''pary'',''parz'']: [x[*]z,y[*]z,Real 0[-]x[**]2[-]y[**]2] && Inv & (x[**]2[+]y[**]2[+]z[**]2[=] Real 1)>) Inv [\<longrightarrow>] Inv"
+lemma allcons4: "\<forall>s. (cons41 [&] cons42 [&] cons43) s"
+  apply (simp add: cons41_def cons42_def cons43_def x_def y_def z_def)
+ by (inv_check_oracle "parz <= 0")
+lemma N4:"{(x [=] Real 1 [&] y [=] Real 0 [&] z [=] Real 0)}
+         <[''parx'',''pary'',''parz'']: [x[*]z,y[*]z,Real 0[-]x[**]2[-]y[**]2] && Inv & (x[**]2[+]y[**]2[+]z[**]2[=] Real 1)>
+          {x [\<le>] Real 1 [&] z[\<le>] Real 0;elE 0 [[|]] almost (x [\<le>] Real 1 [&] z[\<le>] Real 0)}"
+  apply (rule ContinuousRuleGT )
+apply auto
+  apply(simp add:fAnd_def fImp_def fEqual_def)
+      apply (cut_tac allcons4)
+      apply (simp add:fAnd_def fImp_def cons41_def)
+     apply (cut_tac allcons4)
+     apply (simp add:fAnd_def fImp_def cons42_def)
+apply (cut_tac allcons4)
+    apply (simp add:fAnd_def fImp_def cons43_def)
+   apply (simp add:dOr_def)
+  apply(cut_tac allcons4)
+  apply (simp add:fAnd_def fImp_def dOr_def almost_def cons42_def)
+  done
 
+definition cons51 :: fform where "cons51 \<equiv> (x [=] Real 0 [&] y [=] Real (0-1) [&] y[*]a[**]2[=]Real -1) [\<longrightarrow>] Inv"
+definition cons52 :: fform where "cons52 \<equiv> Inv [\<longrightarrow>] ( y[\<le>] Real 0 )"
+definition cons53 :: fform where "cons53 \<equiv> exeFlow(<[''parx'',''pary'',''para'']: [x,y[**]2,Real (1/2)[div]a] && Inv & fTrue>) Inv [\<longrightarrow>] Inv"
+lemma allcons5: "\<forall>s. (cons51 [&] cons52 [&] cons53) s"
+apply (simp only: cons51_def cons52_def cons53_def x_def y_def a_def)
+ by (inv_check_oracle "pary*para^2+1=0")
+
+lemma N5le:"{(x [=] Real 0 [&] y [=] Real (0-1) [&] y[*]a[**]2[=]Real -1)}
+         <[''parx'',''pary'',''para'']: [x,y[**]2,Real (1/2)[div]a] && Inv & fTrue>
+          {( y[\<le>] Real 0 );elE 0 [[|]] almost ( y[\<le>] Real 0 )}"
+  apply (rule ContinuousRuleGT )
+apply auto
+      apply (cut_tac allcons5)
+      apply (simp add:fAnd_def fImp_def cons51_def)
+     apply (cut_tac allcons5)
+     apply (simp add:fAnd_def fImp_def cons52_def)
+apply (cut_tac allcons5)
+    apply (simp add:fAnd_def fImp_def cons53_def)
+   apply (simp add:dOr_def)
+  apply(cut_tac allcons5)
+  apply (simp add:fAnd_def fImp_def dOr_def almost_def cons52_def)
+  done
+lemma N5:"{(x [=] Real 0 [&] y [=] Real (0-1) )}
+         <[''parx'',''pary'']: [x,y[**]2] && Inv & fTrue>
+          {( y[\<le>] Real 0);elE 0 [[|]] almost ( y[\<le>] Real 0)}"
+apply (rule GhostRule[where w="''para''"
+                          and F="Real (1/2)[div]a"
+                          and pre="x [=] Real 0 [&] y [=] Real (0-1) [&] y[*]a[**]2[=]Real -1"
+                          and post="( y[\<le>] Real 0 )"
+                          and HF="(elE 0)[[|]]almost (( y[\<le>] Real 0 ))"])
+         apply auto
+apply(simp add: fAnd_def  fEqual_def  not_in_fform_def x_def y_def )
+   apply(simp add: fLessEqual_def fOr_def fEqual_def fLess_def fGreater_def fNot_def not_in_fform_def x_def y_def ) 
+  apply(simp add:dOr_def   fGreaterEqual_def fLessEqual_def fOr_def fImp_def fEqual_def fLess_def fGreater_def fNot_def not_in_dform_def x_def y_def  almost_def)
+  apply(subgoal_tac "{(x [=] Real 0 [&] y [=] Real (0-1) [&] y[*]a[**]2[=]Real -1)}
+         <[''parx'',''pary'',''para'']: [x,y[**]2,Real (1/2)[div]a] && Inv & fTrue>
+          {( y[\<le>] Real 0 );elE 0 [[|]] almost ( y[\<le>] Real 0 )}")
+  apply(simp add: dOr_def)
+     apply (rule N5le)
+  subgoal for s
+  proof -
+    have not_a: "not_in_fform ''para'' (x [=] Real 0 [&] y [=] Real - 1)"
+      by (simp add: fAnd_def fGreaterEqual_def fLessEqual_def fOr_def fImp_def fEqual_def fLess_def fGreater_def fNot_def not_in_fform_def x_def y_def )
+    have eq: "(x [=] Real 0 [&] y [=] Real - 1) (\<lambda>y. if y \<noteq> ''para'' then s y else  sqrt ( -1/s ''pary'')) \<longleftrightarrow> (x [=] Real 0 [&] y [=] Real - 1) s"
+      by (simp add: not_in_fform_update[OF not_a])
+    show ?thesis
+      apply (rule exI[where x="sqrt ( -1/s ''pary'')"] )
+      apply (auto simp add: eq fAnd_def   fEqual_def fLess_def   x_def y_def  a_def)
+      done
+  qed
+ subgoal for s
+   proof -
+     have not_a: "not_in_fform ''para'' (y [\<le>] Real 0)"
+       by(simp add:  fLessEqual_def fOr_def fImp_def fEqual_def fLess_def fGreater_def fNot_def not_in_fform_def x_def y_def )
+     have eq: "(y [\<le>] Real 0) (\<lambda>y. if y \<noteq> ''para'' then s y else sqrt ( -s ''pary'')) \<longleftrightarrow> (y [\<le>] Real 0) s"
+      by (simp add: not_in_fform_update[OF not_a])
+    show ?thesis
+      apply (rule exI[where x="sqrt ( -s ''pary'')"])
+      apply ( simp add: eq fAnd_def  fLessEqual_def fOr_def fImp_def fEqual_def fLess_def fGreater_def fNot_def  x_def y_def  a_def)
+      done
+  qed
+  subgoal for h n d
+    apply(simp add:dOr_def almost_def fAnd_def a_def )
+    apply (case_tac "n=d")
+    apply auto
+    apply (case_tac "n>d")
+     apply auto
+    apply (case_tac "n<d")
+     apply auto
+    apply (rule exI[where x="\<lambda>t y. sqrt(- (h t  ''pary''))"])
+    apply auto
+      apply (subgoal_tac "not_in_fform ''para'' (y [\<le>] Real 0)")
+       apply(simp add:not_in_fform_def)
+       apply smt
+    apply(simp add:  fLessEqual_def fOr_def fImp_def fEqual_def fLess_def fGreater_def fNot_def not_in_fform_def x_def y_def )
+    apply(simp add:  fLessEqual_def fOr_def fImp_def fEqual_def fLess_def fGreater_def fNot_def  x_def y_def )
+    done
+  done
 
 end
